hpaxos_aux.thy
@@ -1,0 +1,1885 @@
+theory hpaxos_aux
+imports Main hpaxos hpaxos_safety
+begin
+
+
+lemma next_msgs_preserved:
+  assumes "Next st st2"
+      and "x \<in> set (msgs st)"
+  shows "x \<in> set (msgs st2)"
+proof -
+  have css: "ProposerSendAction st st2 \<or>
+        (\<exists>A :: Acceptor. is_safe A
+                    \<and> queued_msg st A = None 
+                    \<and> (\<exists>m \<in> set (msgs st). Process1a A m st st2)) \<or>
+        (\<exists>A :: Acceptor. is_safe A
+                      \<and> queued_msg st A \<noteq> None 
+                      \<and> Process1b A (the (queued_msg st A)) st st2) \<or>
+        (\<exists>A :: Acceptor. is_safe A
+                      \<and> queued_msg st A = None 
+                      \<and> (\<exists>m \<in> set (msgs st). Process1b A m st st2)) \<or>
+        (\<exists>A :: Acceptor. is_safe A
+                      \<and> two_a_lrn_loop st A 
+                      \<and> (\<exists>l :: Learner. Process1bLearnerLoopStep A l st st2)) \<or>
+        (\<exists>A :: Acceptor. is_safe A
+                      \<and> two_a_lrn_loop st A 
+                      \<and> Process1bLearnerLoopDone A st st2) \<or>
+        LearnerProcessAction st st2 \<or>
+        (\<exists>A :: Acceptor. \<not> (is_safe A)
+                      \<and> FakeSend1b A st st2) \<or>
+        (\<exists>A :: Acceptor. \<not> (is_safe A)
+                      \<and> FakeSend2a A st st2)
+        "
+        using assms next_split by presburger
+    then show ?thesis
+    proof (elim disjE)
+      assume "ProposerSendAction st st2"
+      then show ?thesis
+        using assms(2) by auto
+    next
+      assume "\<exists>A. is_safe A \<and>
+                queued_msg st A = None \<and>
+                (\<exists>m\<in>set (msgs st).
+                    Process1a A m st st2)"
+      show ?thesis
+        by (metis Process1a.elims(2) Send.elims(2) \<open>\<exists>A. is_safe A \<and> queued_msg st A = None \<and> (\<exists>m\<in>set (msgs st). Process1a A m st st2)\<close> assms(2) in_set_member member_rec(1))
+    next
+      assume "\<exists>A :: Acceptor. is_safe A
+                        \<and> queued_msg st A \<noteq> None 
+                        \<and> Process1b A (the (queued_msg st A)) st st2"
+      then show ?thesis
+        by (metis Process1b.elims(2) assms(2))
+    next
+      assume "\<exists>A :: Acceptor. is_safe A
+                  \<and> queued_msg st A = None 
+                  \<and> (\<exists>m \<in> set (msgs st). Process1b A m st st2)"
+      then show ?thesis
+        by (metis Process1b.elims(2) assms(2))
+    next
+      assume "\<exists>A :: Acceptor. is_safe A
+                        \<and> two_a_lrn_loop st A 
+                        \<and> (\<exists>l :: Learner. Process1bLearnerLoopStep A l st st2)"
+      then show ?thesis
+        by (metis Process1bLearnerLoopStep.elims(2) Send.elims(2) assms(2) in_set_member member_rec(1))
+    next
+      assume "\<exists>A. is_safe A \<and>
+        two_a_lrn_loop st A \<and>
+        Process1bLearnerLoopDone A st st2"
+      show ?thesis
+        using \<open>\<exists>A. is_safe A \<and> two_a_lrn_loop st A \<and> Process1bLearnerLoopDone A st st2\<close> assms(2) by force
+    next
+      assume "LearnerProcessAction st st2"
+      then show ?thesis
+        by (metis (no_types, lifting) LearnerProcessAction.elims(2) LearnerAction.elims(2) LearnerDecide.elims(2) LearnerRecv.elims(2) assms(2) simps(1) surjective update_convs(3) update_convs(8))
+    next
+      assume "\<exists>A. \<not> is_safe A \<and> FakeSend1b A st st2"
+      show ?thesis
+        by (metis FakeSend1b.simps \<open>\<exists>A. \<not> is_safe A \<and> FakeSend1b A st st2\<close> assms(2) in_set_member member_rec(1) simps(1) surjective update_convs(1))
+    next
+      assume "\<exists>A. \<not> is_safe A \<and> FakeSend2a A st st2"
+      then show ?thesis
+        by (metis FakeSend2a.simps assms(2) ext_inject in_set_member member_rec(1) surjective update_convs(1))
+    qed
+qed
+
+lemma spec_msgs_preserved:
+  assumes "Spec f"
+      and "x \<in> set (msgs (f i))"
+  shows "x \<in> set (msgs (f (i + 1)))"
+  by (metis Spec.elims(2) Suc_eq_plus1 assms(1) assms(2) next_msgs_preserved)
+
+lemma msgs_preserved:
+  assumes "Spec f"
+  shows "j \<ge> i \<longrightarrow> x \<in> set (msgs (f i)) \<longrightarrow> x \<in> set (msgs (f j))"
+proof (induction j)
+  case 0
+  then show ?case
+    by simp
+next
+  case (Suc j)
+  then show ?case
+    by (metis One_nat_def add.right_neutral add_Suc_right assms le_SucE spec_msgs_preserved)
+qed
+
+lemma msgs_preserved_subset:
+  assumes "Spec f"
+      and "i \<le> j"
+  shows "set (msgs (f i)) \<subseteq> set (msgs (f j))"
+  using assms msgs_preserved by blast
+
+lemma next_known_msgs_acc_preserved:
+  assumes "Next st st2"
+      and "x \<in> set (known_msgs_acc st a)"
+    shows "x \<in> set (known_msgs_acc st2 a)"
+proof -
+  have css: "ProposerSendAction st st2 \<or>
+        (\<exists>A :: Acceptor. is_safe A
+                    \<and> queued_msg st A = None 
+                    \<and> (\<exists>m \<in> set (msgs st). Process1a A m st st2)) \<or>
+        (\<exists>A :: Acceptor. is_safe A
+                      \<and> queued_msg st A \<noteq> None 
+                      \<and> Process1b A (the (queued_msg st A)) st st2) \<or>
+        (\<exists>A :: Acceptor. is_safe A
+                      \<and> queued_msg st A = None 
+                      \<and> (\<exists>m \<in> set (msgs st). Process1b A m st st2)) \<or>
+        (\<exists>A :: Acceptor. is_safe A
+                      \<and> two_a_lrn_loop st A 
+                      \<and> (\<exists>l :: Learner. Process1bLearnerLoopStep A l st st2)) \<or>
+        (\<exists>A :: Acceptor. is_safe A
+                      \<and> two_a_lrn_loop st A 
+                      \<and> Process1bLearnerLoopDone A st st2) \<or>
+        LearnerProcessAction st st2 \<or>
+        (\<exists>A :: Acceptor. \<not> (is_safe A)
+                      \<and> FakeSend1b A st st2) \<or>
+        (\<exists>A :: Acceptor. \<not> (is_safe A)
+                      \<and> FakeSend2a A st st2)
+        "
+        using assms next_split by presburger
+    then show ?thesis
+    proof (elim disjE)
+      assume "ProposerSendAction st st2"
+      then show ?thesis
+        using assms(2) by auto
+    next
+      assume "\<exists>A. is_safe A \<and>
+                queued_msg st A = None \<and>
+                (\<exists>m\<in>set (msgs st).
+                    Process1a A m st st2)"
+      show ?thesis
+        by (metis Process1a.elims(2) Store_acc.elims(2) \<open>\<exists>A. is_safe A \<and> queued_msg st A = None \<and> (\<exists>m\<in>set (msgs st). Process1a A m st st2)\<close> assms(2) list.set_intros(2))
+    next
+      assume "\<exists>A :: Acceptor. is_safe A
+                        \<and> queued_msg st A \<noteq> None 
+                        \<and> Process1b A (the (queued_msg st A)) st st2"
+      then show ?thesis
+      proof (clarify)
+        fix A y2
+        assume "is_safe A"
+           and "queued_msg st A = Some y2"
+           and "Process1b A (the (queued_msg st A)) st st2"
+        then have "known_msgs_acc st2 = (
+                \<lambda>x. if A = x 
+                    then y2 # known_msgs_acc st x
+                    else known_msgs_acc st x
+            )"
+          by (metis Process1b.elims(2) Store_acc.elims(2) option.sel)
+        then show ?thesis
+          by (simp add: assms(2))
+      qed
+    next
+      assume "\<exists>A :: Acceptor. is_safe A
+                  \<and> queued_msg st A = None 
+                  \<and> (\<exists>m \<in> set (msgs st). Process1b A m st st2)"
+      then show ?thesis
+      proof (clarify)
+        fix A m
+        assume "is_safe A"
+           and "queued_msg st A = None"
+           and "m \<in> set (msgs st)"
+           and "Process1b A m st st2"
+        then have "known_msgs_acc st2 = (
+                \<lambda>x. if A = x 
+                    then m # known_msgs_acc st x
+                    else known_msgs_acc st x
+            )"
+          by (metis Process1b.elims(2) Store_acc.elims(2))
+        then show ?thesis
+          by (simp add: assms(2))
+      qed
+    next
+      assume "\<exists>A :: Acceptor. is_safe A
+                        \<and> two_a_lrn_loop st A 
+                        \<and> (\<exists>l :: Learner. Process1bLearnerLoopStep A l st st2)"
+      then show ?thesis
+        by (metis Process1bLearnerLoopStep.elims(2) Store_acc.elims(2) assms(2) list.set_intros(2))
+    next
+      assume "\<exists>A. is_safe A \<and>
+        two_a_lrn_loop st A \<and>
+        Process1bLearnerLoopDone A st st2"
+      show ?thesis
+        using \<open>\<exists>A. is_safe A \<and> two_a_lrn_loop st A \<and> Process1bLearnerLoopDone A st st2\<close> assms(2) by force
+    next
+      assume "LearnerProcessAction st st2"
+      then show ?thesis
+        by (smt (verit) LearnerAction.elims(2) LearnerDecide.elims(2) LearnerProcessAction.elims(1) LearnerRecv.elims(2) assms(2) ext_inject surjective update_convs(3) update_convs(8))
+    next
+      assume "\<exists>A. \<not> is_safe A \<and> FakeSend1b A st st2"
+      show ?thesis
+        by (metis FakeSend1b.elims(1) \<open>\<exists>A. \<not> is_safe A \<and> FakeSend1b A st st2\<close> assms(2) ext_inject surjective update_convs(1))
+    next
+      assume "\<exists>A. \<not> is_safe A \<and> FakeSend2a A st st2"
+      then show ?thesis
+        by (metis FakeSend2a.simps assms(2) ext_inject surjective update_convs(1))
+    qed
+qed
+
+lemma known_msgs_acc_preserved:
+  assumes "Spec f"
+  shows "j \<ge> i \<longrightarrow> x \<in> set (known_msgs_acc (f i) a) \<longrightarrow> x \<in> set (known_msgs_acc (f j) a)"
+proof (induction j)
+  case 0
+  then show ?case
+    by simp
+next
+  case (Suc j)
+  then show ?case
+    by (metis Spec.elims(2) assms le_SucE next_known_msgs_acc_preserved)
+qed
+
+lemma known_msgs_acc_preserved_subset:
+  assumes "Spec f"
+      and "i \<le> j"
+  shows "set (known_msgs_acc (f i) a) \<subseteq> set (known_msgs_acc (f j) a)"
+  using assms known_msgs_acc_preserved by blast
+
+
+
+
+
+
+lemma next_known_msgs_lrn_preserved:
+  assumes "Next st st2"
+      and "x \<in> set (known_msgs_lrn st a)"
+    shows "x \<in> set (known_msgs_lrn st2 a)"
+proof -
+  have css: "ProposerSendAction st st2 \<or>
+        (\<exists>A :: Acceptor. is_safe A
+                    \<and> queued_msg st A = None 
+                    \<and> (\<exists>m \<in> set (msgs st). Process1a A m st st2)) \<or>
+        (\<exists>A :: Acceptor. is_safe A
+                      \<and> queued_msg st A \<noteq> None 
+                      \<and> Process1b A (the (queued_msg st A)) st st2) \<or>
+        (\<exists>A :: Acceptor. is_safe A
+                      \<and> queued_msg st A = None 
+                      \<and> (\<exists>m \<in> set (msgs st). Process1b A m st st2)) \<or>
+        (\<exists>A :: Acceptor. is_safe A
+                      \<and> two_a_lrn_loop st A 
+                      \<and> (\<exists>l :: Learner. Process1bLearnerLoopStep A l st st2)) \<or>
+        (\<exists>A :: Acceptor. is_safe A
+                      \<and> two_a_lrn_loop st A 
+                      \<and> Process1bLearnerLoopDone A st st2) \<or>
+        LearnerProcessAction st st2 \<or>
+        (\<exists>A :: Acceptor. \<not> (is_safe A)
+                      \<and> FakeSend1b A st st2) \<or>
+        (\<exists>A :: Acceptor. \<not> (is_safe A)
+                      \<and> FakeSend2a A st st2)
+        "
+        using assms next_split by presburger
+    then show ?thesis
+    proof (elim disjE)
+      assume "ProposerSendAction st st2"
+      then show ?thesis
+        using assms(2) by auto
+    next
+      assume "\<exists>A. is_safe A \<and>
+                queued_msg st A = None \<and>
+                (\<exists>m\<in>set (msgs st).
+                    Process1a A m st st2)"
+      show ?thesis
+        by (metis Process1a.elims(2) Store_acc.elims(2) \<open>\<exists>A. is_safe A \<and> queued_msg st A = None \<and> (\<exists>m\<in>set (msgs st). Process1a A m st st2)\<close> assms(2))
+    next
+      assume "\<exists>A :: Acceptor. is_safe A
+                        \<and> queued_msg st A \<noteq> None 
+                        \<and> Process1b A (the (queued_msg st A)) st st2"
+      then show ?thesis
+      proof (clarify)
+        fix A y2
+        assume "is_safe A"
+           and "queued_msg st A = Some y2"
+           and "Process1b A (the (queued_msg st A)) st st2"
+        then show ?thesis
+          by (simp add: assms(2))
+      qed
+    next
+      assume "\<exists>A :: Acceptor. is_safe A
+                  \<and> queued_msg st A = None 
+                  \<and> (\<exists>m \<in> set (msgs st). Process1b A m st st2)"
+      then show ?thesis
+      proof (clarify)
+        fix A m
+        assume "is_safe A"
+           and "queued_msg st A = None"
+           and "m \<in> set (msgs st)"
+           and "Process1b A m st st2"
+        then show ?thesis
+          by (simp add: assms(2))
+      qed
+    next
+      assume "\<exists>A :: Acceptor. is_safe A
+                        \<and> two_a_lrn_loop st A 
+                        \<and> (\<exists>l :: Learner. Process1bLearnerLoopStep A l st st2)"
+      then show ?thesis
+        by (metis Process1bLearnerLoopStep.elims(2) Store_acc.elims(2) assms(2))
+    next
+      assume "\<exists>A. is_safe A \<and>
+        two_a_lrn_loop st A \<and>
+        Process1bLearnerLoopDone A st st2"
+      show ?thesis
+        using \<open>\<exists>A. is_safe A \<and> two_a_lrn_loop st A \<and> Process1bLearnerLoopDone A st st2\<close> assms(2) by force
+    next
+      assume "LearnerProcessAction st st2"
+      then show ?thesis
+        by (smt (verit) LearnerAction.elims(2) LearnerDecide.elims(2) LearnerProcessAction.elims(1) LearnerRecv.elims(2) assms(2) ext_inject list.set_intros(2) surjective update_convs(3) update_convs(8))
+    next
+      assume "\<exists>A. \<not> is_safe A \<and> FakeSend1b A st st2"
+      show ?thesis
+        by (metis FakeSend1b.elims(1) \<open>\<exists>A. \<not> is_safe A \<and> FakeSend1b A st st2\<close> assms(2) ext_inject surjective update_convs(1))
+    next
+      assume "\<exists>A. \<not> is_safe A \<and> FakeSend2a A st st2"
+      then show ?thesis
+        by (metis FakeSend2a.simps assms(2) ext_inject surjective update_convs(1))
+    qed
+qed
+
+lemma known_msgs_lrn_preserved:
+  assumes "Spec f"
+  shows "j \<ge> i \<longrightarrow> x \<in> set (known_msgs_lrn (f i) a) \<longrightarrow> x \<in> set (known_msgs_lrn (f j) a)"
+proof (induction j)
+  case 0
+  then show ?case
+    by simp
+next
+  case (Suc j)
+  then show ?case
+    by (metis Spec.elims(2) assms le_SucE next_known_msgs_lrn_preserved)
+qed
+
+lemma known_msgs_lrn_preserved_subset:
+  assumes "Spec f"
+      and "i \<le> j"
+  shows "set (known_msgs_lrn (f i) a) \<subseteq> set (known_msgs_lrn (f j) a)"
+  using assms known_msgs_lrn_preserved by blast
+
+
+
+
+
+
+
+
+lemma Next_Preservation:
+  assumes "Spec f"
+      and "\<forall>st st2. Next st st2 \<longrightarrow> P st \<longrightarrow> P st2"
+    shows "j \<ge> i \<longrightarrow> P (f i) \<longrightarrow> P (f j)"
+proof (induction j)
+  case 0
+  then show ?case 
+    by auto
+next
+  case (Suc j)
+  then show ?case
+    by (metis Spec.elims(2) assms(1) assms(2) le_SucE)
+qed
+
+
+lemma Process1a_Not_Process1bLearnerLoopStep:
+  assumes "Process1a a ln st st2"
+  shows "\<not> Process1bLearnerLoopStep a2 ln2 st st2"
+proof -
+  define new1b where "new1b = M1b a (ln # recent_msgs st a)"
+  then show ?thesis
+  proof (cases "WellFormed st new1b")
+    case True
+    then show ?thesis
+      by (smt (verit) PreMessage.distinct(5) Process1a.elims(2) Process1bLearnerLoopStep.elims(2) Send.elims(1) assms list.inject not_Cons_self2)
+  next
+    case False
+    then show ?thesis
+      by (metis Process1a.elims(2) Process1bLearnerLoopStep.elims(2) Send.elims(1) assms new1b_def not_Cons_self2)
+  qed
+qed
+
+
+lemma Wellformed_Conservation_Next:
+  assumes "Next st st2"
+      and "WellFormed st m"
+    shows "WellFormed st2 m"
+proof -
+  have css: "ProposerSendAction st st2 \<or>
+                (\<exists>A :: Acceptor. is_safe A
+                            \<and> queued_msg st A = None 
+                            \<and> (\<exists>m \<in> set (msgs st). Process1a A m st st2)) \<or>
+                (\<exists>A :: Acceptor. is_safe A
+                              \<and> queued_msg st A \<noteq> None 
+                              \<and> Process1b A (the (queued_msg st A)) st st2) \<or>
+                (\<exists>A :: Acceptor. is_safe A
+                              \<and> queued_msg st A = None 
+                              \<and> (\<exists>m \<in> set (msgs st). Process1b A m st st2)) \<or>
+                (\<exists>A :: Acceptor. is_safe A
+                              \<and> two_a_lrn_loop st A 
+                              \<and> (\<exists>l :: Learner. Process1bLearnerLoopStep A l st st2)) \<or>
+                (\<exists>A :: Acceptor. is_safe A
+                              \<and> two_a_lrn_loop st A 
+                              \<and> Process1bLearnerLoopDone A st st2) \<or>
+                LearnerProcessAction st st2 \<or>
+                (\<exists>A :: Acceptor. \<not> (is_safe A)
+                              \<and> FakeSend1b A st st2) \<or>
+                (\<exists>A :: Acceptor. \<not> (is_safe A)
+                              \<and> FakeSend2a A st st2)
+                "
+                using assms next_split by presburger
+    then show ?thesis
+    proof (elim disjE)
+      assume "ProposerSendAction st st2"
+      then show ?thesis
+        using assms(2) by auto
+    next
+      assume "\<exists>A. is_safe A \<and>
+                queued_msg st A = None \<and>
+                (\<exists>m\<in>set (msgs st).
+                    Process1a A m st st2)"
+      then show ?thesis
+        by (metis Process1a.elims(2) WellFormed_monotone assms(2))
+    next
+      assume "\<exists>A :: Acceptor. is_safe A
+                        \<and> queued_msg st A \<noteq> None 
+                        \<and> Process1b A (the (queued_msg st A)) st st2"
+      then show ?thesis
+      proof -
+        show ?thesis
+          using \<open>\<exists>A. is_safe A \<and> queued_msg st A \<noteq> None \<and> Process1b A (the (queued_msg st A)) st st2\<close> assms(2) by force
+      qed
+    next
+      assume "\<exists>A :: Acceptor. is_safe A
+                  \<and> queued_msg st A = None 
+                  \<and> (\<exists>m \<in> set (msgs st). Process1b A m st st2)"
+      then show ?thesis
+      proof -
+        show ?thesis
+          using \<open>\<exists>A. is_safe A \<and> queued_msg st A = None \<and> (\<exists>m\<in>set (msgs st). Process1b A m st st2)\<close> assms(2) by fastforce
+      qed
+    next
+      assume "\<exists>A :: Acceptor. is_safe A
+                        \<and> two_a_lrn_loop st A 
+                        \<and> (\<exists>l :: Learner. Process1bLearnerLoopStep A l st st2)"
+      then show ?thesis
+        by (metis Process1bLearnerLoopStep.elims(2) WellFormed_monotone assms(2))
+    next
+      assume "\<exists>A. is_safe A \<and>
+        two_a_lrn_loop st A \<and>
+        Process1bLearnerLoopDone A st st2"
+      then show ?thesis
+        using assms(2) by auto
+    next
+      assume "LearnerProcessAction st st2"
+      then show ?thesis
+        by (metis (no_types, lifting) LearnerProcessAction.simps LearnerAction.simps LearnerDecide.elims(2) LearnerRecv.elims(2) WellFormed_monotone assms(2) ext_inject surjective update_convs(3) update_convs(8))
+    next
+      assume "\<exists>A. \<not> is_safe A \<and> FakeSend1b A st st2"
+      show ?thesis
+        by (metis FakeSend1b.simps WellFormed_monotone \<open>\<exists>A. \<not> is_safe A \<and> FakeSend1b A st st2\<close> assms(2) ext_inject surjective update_convs(1))
+    next
+      assume "\<exists>A. \<not> is_safe A \<and> FakeSend2a A st st2"
+      then show ?thesis
+        by (metis FakeSend2a.simps WellFormed_monotone assms(2) select_convs(9) surjective update_convs(1))
+    qed
+qed
+
+lemma Wellformed_Conservation:
+  assumes "Spec f"
+      and "WellFormed (f i) m"
+    shows "j \<ge> i \<longrightarrow> WellFormed (f j) m"
+proof (induction j)
+  case 0
+  then show ?case 
+    using assms(2) by blast
+next
+  case (Suc j)
+  then show ?case
+    by (metis Spec.elims(2) Wellformed_Conservation_Next assms(1) assms(2) le_SucE)
+qed
+
+
+
+lemma decision_Conservation_Next:
+  assumes "Next st st2"
+      and "v \<in> decision st L BB"
+    shows "v \<in> decision st2 L BB"
+proof -
+  have css: "ProposerSendAction st st2 \<or>
+                (\<exists>A :: Acceptor. is_safe A
+                            \<and> queued_msg st A = None 
+                            \<and> (\<exists>m \<in> set (msgs st). Process1a A m st st2)) \<or>
+                (\<exists>A :: Acceptor. is_safe A
+                              \<and> queued_msg st A \<noteq> None 
+                              \<and> Process1b A (the (queued_msg st A)) st st2) \<or>
+                (\<exists>A :: Acceptor. is_safe A
+                              \<and> queued_msg st A = None 
+                              \<and> (\<exists>m \<in> set (msgs st). Process1b A m st st2)) \<or>
+                (\<exists>A :: Acceptor. is_safe A
+                              \<and> two_a_lrn_loop st A 
+                              \<and> (\<exists>l :: Learner. Process1bLearnerLoopStep A l st st2)) \<or>
+                (\<exists>A :: Acceptor. is_safe A
+                              \<and> two_a_lrn_loop st A 
+                              \<and> Process1bLearnerLoopDone A st st2) \<or>
+                LearnerProcessAction st st2 \<or>
+                (\<exists>A :: Acceptor. \<not> (is_safe A)
+                              \<and> FakeSend1b A st st2) \<or>
+                (\<exists>A :: Acceptor. \<not> (is_safe A)
+                              \<and> FakeSend2a A st st2)
+                "
+                using assms next_split by presburger
+    then show ?thesis
+    proof (elim disjE)
+      assume "ProposerSendAction st st2"
+      then show ?thesis
+        using assms(2) by auto
+    next
+      assume "\<exists>A. is_safe A \<and>
+                queued_msg st A = None \<and>
+                (\<exists>m\<in>set (msgs st).
+                    Process1a A m st st2)"
+      then show ?thesis
+        by (metis Process1a.elims(2) assms(2))
+    next
+      assume "\<exists>A :: Acceptor. is_safe A
+                        \<and> queued_msg st A \<noteq> None 
+                        \<and> Process1b A (the (queued_msg st A)) st st2"
+      then show ?thesis
+      proof -
+        show ?thesis
+          using \<open>\<exists>A. is_safe A \<and> queued_msg st A \<noteq> None \<and> Process1b A (the (queued_msg st A)) st st2\<close> assms(2) by force
+      qed
+    next
+      assume "\<exists>A :: Acceptor. is_safe A
+                  \<and> queued_msg st A = None 
+                  \<and> (\<exists>m \<in> set (msgs st). Process1b A m st st2)"
+      then show ?thesis
+      proof -
+        show ?thesis
+          using \<open>\<exists>A. is_safe A \<and> queued_msg st A = None \<and> (\<exists>m\<in>set (msgs st). Process1b A m st st2)\<close> assms(2) by fastforce
+      qed
+    next
+      assume "\<exists>A :: Acceptor. is_safe A
+                        \<and> two_a_lrn_loop st A 
+                        \<and> (\<exists>l :: Learner. Process1bLearnerLoopStep A l st st2)"
+      then show ?thesis
+        by (metis Process1bLearnerLoopStep.elims(2) assms(2))
+    next
+      assume "\<exists>A. is_safe A \<and>
+        two_a_lrn_loop st A \<and>
+        Process1bLearnerLoopDone A st st2"
+      then show ?thesis
+        using assms(2) by auto
+    next
+      assume "LearnerProcessAction st st2"
+      then show ?thesis
+        unfolding LearnerProcessAction.simps LearnerAction.simps
+      proof (clarify)
+        fix ln
+        assume "(\<exists>m\<in>set (msgs st). LearnerRecv ln m st st2) \<or>
+              (\<exists>blt val. LearnerDecide ln blt val st st2)"
+        then show ?thesis
+        proof (elim disjE; clarify)
+          fix m
+          assume "m \<in> set (msgs st)"
+             and "LearnerRecv ln m st st2"
+          then show ?thesis
+            by (simp add: assms(2) surjective)
+          next
+            fix blt val
+            assume "LearnerDecide ln blt val st st2"
+            show ?thesis
+            using \<open>LearnerDecide ln blt val st st2\<close> assms(2) by force
+        qed
+      qed
+    next
+      assume "\<exists>A. \<not> is_safe A \<and> FakeSend1b A st st2"
+      show ?thesis
+        by (metis FakeSend1b.simps \<open>\<exists>A. \<not> is_safe A \<and> FakeSend1b A st st2\<close> assms(2) ext_inject surjective update_convs(1))
+    next
+      assume "\<exists>A. \<not> is_safe A \<and> FakeSend2a A st st2"
+      then show ?thesis
+        by (metis FakeSend2a.simps assms(2) ext_inject surjective update_convs(1))
+    qed
+qed
+
+lemma decision_Conservation:
+  assumes "Spec f"
+      and "v \<in> decision (f i) L BB"
+    shows "j \<ge> i \<longrightarrow> v \<in> decision (f j) L BB"
+proof (induction j)
+  case 0
+  then show ?case 
+    using assms(2) by blast
+next
+  case (Suc j)
+  then show ?case
+    by (metis Spec.elims(2) decision_Conservation_Next assms(1) assms(2) le_SucE)
+qed
+
+lemma decision_Conservation_subset:
+  assumes "Spec f"
+      and "i \<le> j"
+    shows "decision (f i) L BB \<subseteq> decision (f j) L BB"
+  using assms(1) assms(2) decision_Conservation by blast
+
+fun QueuedMsgSpec2 :: "State \<Rightarrow> bool" where
+  "QueuedMsgSpec2 st = (
+    \<forall>a :: Acceptor. is_safe a \<and> queued_msg st a \<noteq> None \<longrightarrow> 
+      Recv_acc st a (the (queued_msg st a))
+  )"
+
+
+lemma QueuedMsgSpecInvariant2 :
+  assumes "QueuedMsgSpec2 st"
+      and "Next st st2"
+      and "FullSafetyInvariant st"
+  shows "QueuedMsgSpec2 st2"
+  unfolding QueuedMsgSpec2.simps Recv_acc.simps
+proof (clarify)
+  fix a y
+  assume "is_safe a"
+     and "queued_msg st2 a = Some y"
+  have css: "ProposerSendAction st st2 \<or>
+                (\<exists>A :: Acceptor. is_safe A
+                            \<and> queued_msg st A = None 
+                            \<and> (\<exists>m \<in> set (msgs st). Process1a A m st st2)) \<or>
+                (\<exists>A :: Acceptor. is_safe A
+                              \<and> queued_msg st A \<noteq> None 
+                              \<and> Process1b A (the (queued_msg st A)) st st2) \<or>
+                (\<exists>A :: Acceptor. is_safe A
+                              \<and> queued_msg st A = None 
+                              \<and> (\<exists>m \<in> set (msgs st). Process1b A m st st2)) \<or>
+                (\<exists>A :: Acceptor. is_safe A
+                              \<and> two_a_lrn_loop st A 
+                              \<and> (\<exists>l :: Learner. Process1bLearnerLoopStep A l st st2)) \<or>
+                (\<exists>A :: Acceptor. is_safe A
+                              \<and> two_a_lrn_loop st A 
+                              \<and> Process1bLearnerLoopDone A st st2) \<or>
+                LearnerProcessAction st st2 \<or>
+                (\<exists>A :: Acceptor. \<not> (is_safe A)
+                              \<and> FakeSend1b A st st2) \<or>
+                (\<exists>A :: Acceptor. \<not> (is_safe A)
+                              \<and> FakeSend2a A st st2)
+                "
+                using assms next_split by presburger
+    then show "the (queued_msg st2 a) \<notin> set (known_msgs_acc st2 a) \<and>
+               WellFormed st2 (the (queued_msg st2 a)) \<and>
+               Proper_acc st2 a (the (queued_msg st2 a))"
+    proof (elim disjE)
+      assume "ProposerSendAction st st2"
+      then show ?thesis
+        by (smt (verit) Proper_acc.elims(2) Proper_acc.elims(3) ProposerSendAction.elims(2) QueuedMsgSpec2.simps Recv_acc.elims(1) Send1a.elims(2) Wellformed_Conservation_Next \<open>is_safe a\<close> \<open>queued_msg st2 a = Some y\<close> assms(1) assms(2) ext_inject not_None_eq surjective update_convs(1))
+    next
+      assume "\<exists>A. is_safe A \<and>
+                queued_msg st A = None \<and>
+                (\<exists>m\<in>set (msgs st).
+                    Process1a A m st st2)"
+      then show ?thesis
+      proof (clarify)
+        fix A m
+        assume "is_safe A"
+           and "queued_msg st A = None"
+           and "m \<in> set (msgs st)"
+           and "Process1a A m st st2"
+        then show ?thesis
+        proof (cases "A = a")
+          case True
+          have h1: "WellFormed st2 (the (queued_msg st2 a))"
+            by (smt (verit, ccfv_threshold) Process1a.elims(2) True Wellformed_Conservation_Next \<open>Process1a A m st st2\<close> \<open>queued_msg st A = None\<close> \<open>queued_msg st2 a = Some y\<close> assms(2) option.discI option.sel)
+          have "y = M1b a (m # recent_msgs st a)"
+            by (smt (verit, best) Process1a.elims(2) True \<open>Process1a A m st st2\<close> \<open>queued_msg st A = None\<close> \<open>queued_msg st2 a = Some y\<close> option.discI option.sel)
+          have "Recv_acc st a m"
+            by (metis Process1a.elims(2) True \<open>Process1a A m st st2\<close>)
+          have "Store_acc a m st st2"
+            by (metis Process1a.elims(2) True \<open>Process1a A m st st2\<close>)
+          have "Send y st st2"
+            by (metis Process1a.elims(2) True \<open>Process1a A m st st2\<close> \<open>queued_msg st A = None\<close> \<open>queued_msg st2 a = Some y\<close> \<open>y = M1b a (m # recent_msgs st a)\<close> option.discI)
+          have "Process1a a m st st2"
+            using \<open>Process1a A m st st2\<close> True by blast
+          have "m \<notin> set (known_msgs_acc st a)"
+            by (meson Recv_acc.elims(2) \<open>Recv_acc st a m\<close>)
+          have "known_msgs_acc st2 a =  m # known_msgs_acc st a"
+            using \<open>Store_acc a m st st2\<close> by auto
+          have "y \<notin> set (known_msgs_acc st a)"
+            by (metis FullSafetyInvariant.elims(2) KnownMsgs_accSpec.elims(2) Proper_acc.elims(2) \<open>is_safe a\<close> \<open>m \<notin> set (known_msgs_acc st a)\<close> \<open>y = M1b a (m # recent_msgs st a)\<close> assms(3) list.set_intros(1) ref.simps(2))
+          have h2: "y \<notin> set (known_msgs_acc st2 a)"
+            by (metis Proper_acc.elims(2) Recv_acc.elims(2) \<open>Recv_acc st a m\<close> \<open>known_msgs_acc st2 a = m # known_msgs_acc st a\<close> \<open>y = M1b a (m # recent_msgs st a)\<close> \<open>y \<notin> set (known_msgs_acc st a)\<close> list.set_intros(1) ref.simps(2) set_ConsD)
+          have h3: "Proper_acc st2 a y"
+            by (metis (no_types, lifting) FullSafetyInvariant.elims(2) Proper_acc.elims(1) RecentMsgsSpec.elims(2) \<open>is_safe a\<close> \<open>known_msgs_acc st2 a = m # known_msgs_acc st a\<close> \<open>y = M1b a (m # recent_msgs st a)\<close> assms(3) insert_iff list.simps(15) ref.simps(2) subsetD)
+          show ?thesis
+            by (metis \<open>queued_msg st2 a = Some y\<close> h1 h2 h3 option.sel)
+        next
+          case False
+          then show ?thesis
+            by (smt (verit) Process1a.elims(2) Proper_acc.elims(2) Proper_acc.elims(3) QueuedMsgSpec2.simps Recv_acc.elims(1) Store_acc.elims(2) Wellformed_Conservation_Next \<open>Process1a A m st st2\<close> \<open>is_safe a\<close> \<open>queued_msg st2 a = Some y\<close> assms(1) assms(2) option.discI)
+        qed
+      qed
+    next
+      assume "\<exists>A :: Acceptor. is_safe A
+                        \<and> queued_msg st A \<noteq> None 
+                        \<and> Process1b A (the (queued_msg st A)) st st2"
+      then show ?thesis
+          unfolding Process1b.simps
+      proof (clarify)
+        fix A y2
+        assume "queued_msg st2 = (\<lambda>x. if x = A then None else queued_msg st x)"
+        have "A \<noteq> a"
+          using \<open>queued_msg st2 = (\<lambda>x. if x = A then None else queued_msg st x)\<close> \<open>queued_msg st2 a = Some y\<close> by auto
+        have "queued_msg st2 a = queued_msg st a"
+          using \<open>A \<noteq> a\<close> \<open>queued_msg st2 = (\<lambda>x. if x = A then None else queued_msg st x)\<close> by presburger
+        have h1: "WellFormed st2 (the (queued_msg st2 a))"
+          by (metis QueuedMsgSpec2.elims(2) Recv_acc.elims(2) Wellformed_Conservation_Next \<open>is_safe a\<close> \<open>queued_msg st2 a = Some y\<close> \<open>queued_msg st2 a = queued_msg st a\<close> assms(1) assms(2) option.discI)
+        have h2: "y \<notin> set (known_msgs_acc st2 a)"
+        proof -
+          obtain aa :: Acceptor where
+            f1: "queued_msg st aa \<noteq> None \<and> Process1b aa (the (queued_msg st aa)) st st2"
+            using \<open>\<exists>A. is_safe A \<and> queued_msg st A \<noteq> None \<and> Process1b A (the (queued_msg st A)) st st2\<close> by blast
+          then have "\<And>a. a \<noteq> aa \<or> queued_msg st2 a = None"
+            by simp
+          then have "aa = A"
+            using f1 by (metis \<open>queued_msg st2 = (\<lambda>x. if x = A then None else queued_msg st x)\<close>)
+          then have "\<And>a. A = a \<or> known_msgs_acc st2 a = known_msgs_acc st a"
+            using f1 by simp
+          then show ?thesis
+            by (metis QueuedMsgSpec2.elims(2) Recv_acc.elims(2) \<open>A \<noteq> a\<close> \<open>is_safe a\<close> \<open>queued_msg st2 a = Some y\<close> \<open>queued_msg st2 a = queued_msg st a\<close> assms(1) option.discI option.sel)
+        qed
+        have h3: "Proper_acc st2 a y"
+          by (metis Proper_acc.elims(1) QueuedMsgSpec2.elims(2) Recv_acc.elims(2) \<open>is_safe a\<close> \<open>queued_msg st2 a = Some y\<close> \<open>queued_msg st2 a = queued_msg st a\<close> assms(1) assms(2) next_known_msgs_acc_preserved option.discI option.sel)
+        show ?thesis
+          by (metis \<open>queued_msg st2 a = Some y\<close> h1 h2 h3 option.sel)
+      qed
+    next
+      assume "\<exists>A :: Acceptor. is_safe A
+                  \<and> queued_msg st A = None 
+                  \<and> (\<exists>m \<in> set (msgs st). Process1b A m st st2)"
+      then show ?thesis
+        unfolding Process1b.simps
+      proof (clarify)
+        fix A m
+        assume "queued_msg st2 = (\<lambda>x. if x = A then None else queued_msg st x)"
+           and "Store_acc A m st st2"
+        have "A \<noteq> a"
+          using \<open>queued_msg st2 = (\<lambda>x. if x = A then None else queued_msg st x)\<close> \<open>queued_msg st2 a = Some y\<close> by auto
+        have "queued_msg st2 a = queued_msg st a"
+          using \<open>A \<noteq> a\<close> \<open>queued_msg st2 = (\<lambda>x. if x = A then None else queued_msg st x)\<close> by presburger
+        have h1: "WellFormed st2 (the (queued_msg st2 a))"
+          by (metis QueuedMsgSpec2.elims(2) Recv_acc.elims(2) Wellformed_Conservation_Next \<open>is_safe a\<close> \<open>queued_msg st2 a = Some y\<close> \<open>queued_msg st2 a = queued_msg st a\<close> assms(1) assms(2) option.discI)
+        have h3: "Proper_acc st2 a y"
+          by (metis Proper_acc.elims(2) Proper_acc.elims(3) QueuedMsgSpec2.simps Recv_acc.elims(2) \<open>is_safe a\<close> \<open>queued_msg st2 a = Some y\<close> \<open>queued_msg st2 a = queued_msg st a\<close> assms(1) assms(2) next_known_msgs_acc_preserved option.distinct(1) option.sel)
+        have h2: "y \<notin> set (known_msgs_acc st2 a)"
+          by (metis QueuedMsgSpec2.elims(2) Recv_acc.elims(2) Store_acc.elims(2) \<open>A \<noteq> a\<close> \<open>Store_acc A m st st2\<close> \<open>is_safe a\<close> \<open>queued_msg st2 a = Some y\<close> \<open>queued_msg st2 a = queued_msg st a\<close> assms(1) option.discI option.sel)
+        show ?thesis
+          by (metis \<open>queued_msg st2 a = Some y\<close> h1 h2 h3 option.sel)
+      qed
+    next
+      assume "\<exists>A :: Acceptor. is_safe A
+                        \<and> two_a_lrn_loop st A 
+                        \<and> (\<exists>l :: Learner. Process1bLearnerLoopStep A l st st2)"
+      then show ?thesis
+        by (smt (verit) FullSafetyInvariant.elims(2) Process1bLearnerLoopStep.elims(2) Proper_acc.elims(1) QueuedMsgSpec2.simps Recv_acc.elims(2) Store_acc.elims(2) Wellformed_Conservation_Next \<open>is_safe a\<close> \<open>queued_msg st2 a = Some y\<close> assms(1) assms(2) assms(3) option.discI twoaLearnerLoopSpec.elims(2))
+    next
+      assume "\<exists>A. is_safe A \<and>
+        two_a_lrn_loop st A \<and>
+        Process1bLearnerLoopDone A st st2"
+      then show ?thesis
+        by (smt (verit) Process1bLearnerLoopDone.elims(1) Proper_acc.elims(1) QueuedMsgSpec2.simps Recv_acc.elims(2) Wellformed_Conservation_Next \<open>is_safe a\<close> \<open>queued_msg st2 a = Some y\<close> assms(1) assms(2) ext_inject option.discI surjective update_convs(6))
+    next
+      assume "LearnerProcessAction st st2"
+      then show ?thesis
+        unfolding LearnerProcessAction.simps LearnerAction.simps
+      proof (clarify)
+        fix ln
+        assume "(\<exists>m\<in>set (msgs st). LearnerRecv ln m st st2) \<or>
+              (\<exists>blt val. LearnerDecide ln blt val st st2)"
+        then show ?thesis
+        proof (elim disjE; clarify)
+          fix m
+          assume "m \<in> set (msgs st)"
+             and "LearnerRecv ln m st st2"
+          then show ?thesis
+            by (smt (verit) LearnerRecv.elims(2) Proper_acc.elims(1) QueuedMsgSpec2.simps Recv_acc.elims(2) Wellformed_Conservation_Next \<open>is_safe a\<close> \<open>queued_msg st2 a = Some y\<close> assms(1) assms(2) option.discI select_convs(2) select_convs(5) surjective update_convs(3))
+          next
+            fix blt val
+            assume "LearnerDecide ln blt val st st2"
+            show ?thesis
+              by (smt (verit) LearnerDecide.elims(2) Proper_acc.elims(1) QueuedMsgSpec2.simps Recv_acc.elims(2) Wellformed_Conservation_Next \<open>LearnerDecide ln blt val st st2\<close> \<open>is_safe a\<close> \<open>queued_msg st2 a = Some y\<close> assms(1) assms(2) ext_inject option.discI surjective update_convs(8))
+        qed
+      qed
+    next
+      assume "\<exists>A. \<not> is_safe A \<and> FakeSend1b A st st2"
+      show ?thesis
+        by (smt (verit) FakeSend1b.elims(1) Proper_acc.elims(1) QueuedMsgSpec2.simps Recv_acc.elims(2) Wellformed_Conservation_Next \<open>\<exists>A. \<not> is_safe A \<and> FakeSend1b A st st2\<close> \<open>is_safe a\<close> \<open>queued_msg st2 a = Some y\<close> assms(1) assms(2) option.discI select_convs(2) select_convs(5) surjective update_convs(1))
+    next
+      assume "\<exists>A. \<not> is_safe A \<and> FakeSend2a A st st2"
+      then show ?thesis
+        by (smt (verit) FakeSend2a.simps Proper_acc.elims(1) QueuedMsgSpec2.simps Recv_acc.elims(1) Wellformed_Conservation_Next \<open>is_safe a\<close> \<open>queued_msg st2 a = Some y\<close> assms(1) assms(2) ext_inject option.discI surjective update_convs(1))
+    qed
+qed
+
+lemma QueuedMsgSpec2_Conserved:
+  assumes "Spec f"
+    shows "QueuedMsgSpec2 (f i)"
+proof (induction i)
+  case 0
+  then show ?case 
+    by (metis Init.elims QueuedMsgResult QueuedMsgSpec1.elims(2) QueuedMsgSpec2.simps Spec.simps assms length_greater_0_conv length_pos_if_in_set select_convs(1))
+next
+  case (Suc j)
+  then show ?case
+    by (metis PreSafetyResult QueuedMsgSpecInvariant2 Spec.elims(2) assms)
+qed
+
+lemma BVal_Doesnt_Change:
+  assumes "Next st st2"
+  shows "BVal st = BVal st2"
+proof -have css: "ProposerSendAction st st2 \<or>
+                (\<exists>A :: Acceptor. is_safe A
+                            \<and> queued_msg st A = None 
+                            \<and> (\<exists>m \<in> set (msgs st). Process1a A m st st2)) \<or>
+                (\<exists>A :: Acceptor. is_safe A
+                              \<and> queued_msg st A \<noteq> None 
+                              \<and> Process1b A (the (queued_msg st A)) st st2) \<or>
+                (\<exists>A :: Acceptor. is_safe A
+                              \<and> queued_msg st A = None 
+                              \<and> (\<exists>m \<in> set (msgs st). Process1b A m st st2)) \<or>
+                (\<exists>A :: Acceptor. is_safe A
+                              \<and> two_a_lrn_loop st A 
+                              \<and> (\<exists>l :: Learner. Process1bLearnerLoopStep A l st st2)) \<or>
+                (\<exists>A :: Acceptor. is_safe A
+                              \<and> two_a_lrn_loop st A 
+                              \<and> Process1bLearnerLoopDone A st st2) \<or>
+                LearnerProcessAction st st2 \<or>
+                (\<exists>A :: Acceptor. \<not> (is_safe A)
+                              \<and> FakeSend1b A st st2) \<or>
+                (\<exists>A :: Acceptor. \<not> (is_safe A)
+                              \<and> FakeSend2a A st st2)
+                "
+    using assms next_split by presburger
+    then show ?thesis
+    proof (elim disjE)
+      assume "ProposerSendAction st st2"
+      then show ?thesis
+        by auto
+    next
+      assume "\<exists>A. is_safe A \<and>
+                queued_msg st A = None \<and>
+                (\<exists>m\<in>set (msgs st).
+                    Process1a A m st st2)"
+      then show ?thesis
+        by (metis Process1a.elims(2))
+    next
+      assume "\<exists>A :: Acceptor. is_safe A
+                        \<and> queued_msg st A \<noteq> None 
+                        \<and> Process1b A (the (queued_msg st A)) st st2"
+      then show ?thesis
+      proof -
+        show ?thesis
+          using \<open>\<exists>A. is_safe A \<and> queued_msg st A \<noteq> None \<and> Process1b A (the (queued_msg st A)) st st2\<close> by force
+      qed
+    next
+      assume "\<exists>A :: Acceptor. is_safe A
+                  \<and> queued_msg st A = None 
+                  \<and> (\<exists>m \<in> set (msgs st). Process1b A m st st2)"
+      then show ?thesis
+      proof -
+        show ?thesis
+          using \<open>\<exists>A. is_safe A \<and> queued_msg st A = None \<and> (\<exists>m\<in>set (msgs st). Process1b A m st st2)\<close> by force
+      qed
+    next
+      assume "\<exists>A :: Acceptor. is_safe A
+                        \<and> two_a_lrn_loop st A 
+                        \<and> (\<exists>l :: Learner. Process1bLearnerLoopStep A l st st2)"
+      then show ?thesis
+        by (metis Process1bLearnerLoopStep.elims(2))
+    next
+      assume "\<exists>A. is_safe A \<and>
+        two_a_lrn_loop st A \<and>
+        Process1bLearnerLoopDone A st st2"
+      then show ?thesis
+        by auto
+    next
+      assume "LearnerProcessAction st st2"
+      then show ?thesis
+        by (smt (verit) LearnerAction.elims(2) LearnerDecide.elims(2) LearnerProcessAction.elims(1) LearnerRecv.elims(2) ext_inject surjective update_convs(3) update_convs(8))
+    next
+      assume "\<exists>A. \<not> is_safe A \<and> FakeSend1b A st st2"
+      show ?thesis
+        by (metis FakeSend1b.elims(2) \<open>\<exists>A. \<not> is_safe A \<and> FakeSend1b A st st2\<close> select_convs(9) surjective update_convs(1))
+    next
+      assume "\<exists>A. \<not> is_safe A \<and> FakeSend2a A st st2"
+      then show ?thesis
+        by (metis FakeSend2a.simps ext_inject surjective update_convs(1))
+      qed
+qed
+
+lemma BVal_Constant_Ord:
+  assumes "Spec f"
+    shows "i \<le> j \<longrightarrow> BVal (f i) = BVal (f j)"
+proof (induction j)
+  case 0
+  then show ?case 
+    by fastforce
+next
+  case (Suc j)
+  then show ?case
+    by (smt (z3) BVal_Doesnt_Change Spec.elims(2) assms le_SucE)
+qed
+
+lemma BVal_Constant:
+  assumes "Spec f"
+    shows "BVal (f i) = BVal (f j)"
+  by (metis BVal_Constant_Ord assms nat_le_linear)
+
+lemma Wellformed_Constant:
+  assumes "Spec f"
+  shows "WellFormed (f i) m = WellFormed (f j) m"
+  using BVal_Constant WellFormed_monotone assms by blast
+
+lemma Choice_Made_Perminent_Next:
+  assumes "ChosenIn st l b v"
+      and "Next st st2"
+    shows "ChosenIn st2 l b v"
+proof -
+  have mq: "known_msgs_lrn st2 l = known_msgs_lrn st l \<longrightarrow> ChosenIn st2 l b v"
+    unfolding ChosenIn.simps Known2a.simps V.simps
+    by (smt (verit) BVal_Doesnt_Change ChosenIn.simps Known2a.simps V.elims(2) assms(1) assms(2) mem_Collect_eq subset_iff)
+  have css: "ProposerSendAction st st2 \<or>
+                (\<exists>A :: Acceptor. is_safe A
+                            \<and> queued_msg st A = None 
+                            \<and> (\<exists>m \<in> set (msgs st). Process1a A m st st2)) \<or>
+                (\<exists>A :: Acceptor. is_safe A
+                              \<and> queued_msg st A \<noteq> None 
+                              \<and> Process1b A (the (queued_msg st A)) st st2) \<or>
+                (\<exists>A :: Acceptor. is_safe A
+                              \<and> queued_msg st A = None 
+                              \<and> (\<exists>m \<in> set (msgs st). Process1b A m st st2)) \<or>
+                (\<exists>A :: Acceptor. is_safe A
+                              \<and> two_a_lrn_loop st A 
+                              \<and> (\<exists>l :: Learner. Process1bLearnerLoopStep A l st st2)) \<or>
+                (\<exists>A :: Acceptor. is_safe A
+                              \<and> two_a_lrn_loop st A 
+                              \<and> Process1bLearnerLoopDone A st st2) \<or>
+                LearnerProcessAction st st2 \<or>
+                (\<exists>A :: Acceptor. \<not> (is_safe A)
+                              \<and> FakeSend1b A st st2) \<or>
+                (\<exists>A :: Acceptor. \<not> (is_safe A)
+                              \<and> FakeSend2a A st st2)
+                "
+                using assms next_split by presburger
+    then show ?thesis
+    proof (elim disjE)
+      assume "ProposerSendAction st st2"
+      then show ?thesis
+        using mq by fastforce
+    next
+      assume "\<exists>A. is_safe A \<and>
+                queued_msg st A = None \<and>
+                (\<exists>m\<in>set (msgs st).
+                    Process1a A m st st2)"
+      then show ?thesis
+        by (metis Process1a.elims(2) Store_acc.elims(2) mq)
+    next
+      assume "\<exists>A :: Acceptor. is_safe A
+                        \<and> queued_msg st A \<noteq> None 
+                        \<and> Process1b A (the (queued_msg st A)) st st2"
+      then show ?thesis
+        by (metis Process1b.elims(2) Store_acc.elims(2) mq)
+    next
+      assume "\<exists>A :: Acceptor. is_safe A
+                  \<and> queued_msg st A = None 
+                  \<and> (\<exists>m \<in> set (msgs st). Process1b A m st st2)"
+      then show ?thesis
+        by (metis Process1b.elims(2) Store_acc.elims(1) mq)
+    next
+      assume "\<exists>A :: Acceptor. is_safe A
+                        \<and> two_a_lrn_loop st A 
+                        \<and> (\<exists>l :: Learner. Process1bLearnerLoopStep A l st st2)"
+      then show ?thesis
+        by (metis Process1bLearnerLoopStep.elims(2) Store_acc.elims(2) mq)
+    next
+      assume "\<exists>A. is_safe A \<and>
+        two_a_lrn_loop st A \<and>
+        Process1bLearnerLoopDone A st st2"
+      then show ?thesis
+        by (smt (z3) Process1bLearnerLoopDone.elims(1) ext_inject mq surjective update_convs(6))
+    next
+      assume "LearnerProcessAction st st2"
+      then show ?thesis
+        unfolding LearnerProcessAction.simps LearnerAction.simps
+      proof (clarify)
+        fix ln
+        assume "(\<exists>m\<in>set (msgs st). LearnerRecv ln m st st2) \<or>
+              (\<exists>blt val. LearnerDecide ln blt val st st2)"
+        then show ?thesis
+        proof (elim disjE; clarify)
+          fix m
+          assume "m \<in> set (msgs st)"
+             and "LearnerRecv ln m st st2"
+          then show ?thesis
+            unfolding LearnerRecv.simps
+          proof (cases "ln = l")
+            case True
+            have "known_msgs_lrn st2 l = m # known_msgs_lrn st l"
+              by (smt (verit, del_insts) LearnerRecv.elims(2) True \<open>LearnerRecv ln m st st2\<close> select_convs(3) surjective update_convs(3))
+            show ?thesis 
+              by (smt (verit) ChosenIn.simps Known2a.simps LearnerRecv.elims(2) V.simps \<open>LearnerRecv ln m st st2\<close> assms(1) ext_inject list.set_intros(2) mem_Collect_eq subset_iff surjective update_convs(3))
+          next
+            case False
+            then show ?thesis
+              by (smt (verit, ccfv_threshold) LearnerRecv.elims(2) \<open>LearnerRecv ln m st st2\<close> ext_inject mq surjective update_convs(3))
+          qed
+          next
+            fix blt val
+            assume "LearnerDecide ln blt val st st2"
+            then show ?thesis
+              by (metis (no_types, lifting) LearnerDecide.elims(2) ext_inject mq surjective update_convs(8))
+        qed
+      qed
+    next
+      assume "\<exists>A. \<not> is_safe A \<and> FakeSend1b A st st2"
+      show ?thesis
+        by (metis FakeSend1b.elims(1) \<open>\<exists>A. \<not> is_safe A \<and> FakeSend1b A st st2\<close> mq select_convs(3) surjective update_convs(1))
+    next
+      assume "\<exists>A. \<not> is_safe A \<and> FakeSend2a A st st2"
+      then show ?thesis
+        by (metis FakeSend2a.simps mq select_convs(3) surjective update_convs(1))
+    qed
+qed
+
+
+lemma Choice_Made_Perminent:
+  assumes "Spec f"
+      and "ChosenIn (f i) l b v"
+    shows "j \<ge> i \<longrightarrow> ChosenIn (f j) l b v"
+proof (induction j)
+  case 0
+  then show ?case 
+    using assms(2) by blast
+next
+  case (Suc j)
+  then show ?case
+    by (metis Choice_Made_Perminent_Next Spec.simps assms(1) assms(2) le_Suc_eq)
+qed
+
+
+lemma M1a_Good:
+  assumes "m \<in> set (msgs st)"
+      and "type m = T1a"
+      and "m \<notin> set (known_msgs_lrn st l)"
+    shows "Proper_lrn st l m"
+  by (metis MessageType.distinct(1) MessageType.distinct(3) Proper_lrn.simps assms(2) empty_iff ref.simps(1) type.elims)
+
+fun Msg_ref_Spec :: "State \<Rightarrow> bool" where
+  "Msg_ref_Spec st = (
+    \<forall>m \<in> set (msgs st). is_safe (acc m) \<longrightarrow> ref m \<subseteq> set (msgs st)
+  )"
+
+lemma Msg_ref_Spec_Next:
+  assumes "Next st st2"
+      and "Msg_ref_Spec st"
+      and "RecentMsgsSpec st"
+      and "KnownMsgs_accSpec st"
+    shows "Msg_ref_Spec st2"
+proof -
+  have css: "ProposerSendAction st st2 \<or>
+                (\<exists>A :: Acceptor. is_safe A
+                            \<and> queued_msg st A = None 
+                            \<and> (\<exists>m \<in> set (msgs st). Process1a A m st st2)) \<or>
+                (\<exists>A :: Acceptor. is_safe A
+                              \<and> queued_msg st A \<noteq> None 
+                              \<and> Process1b A (the (queued_msg st A)) st st2) \<or>
+                (\<exists>A :: Acceptor. is_safe A
+                              \<and> queued_msg st A = None 
+                              \<and> (\<exists>m \<in> set (msgs st). Process1b A m st st2)) \<or>
+                (\<exists>A :: Acceptor. is_safe A
+                              \<and> two_a_lrn_loop st A 
+                              \<and> (\<exists>l :: Learner. Process1bLearnerLoopStep A l st st2)) \<or>
+                (\<exists>A :: Acceptor. is_safe A
+                              \<and> two_a_lrn_loop st A 
+                              \<and> Process1bLearnerLoopDone A st st2) \<or>
+                LearnerProcessAction st st2 \<or>
+                (\<exists>A :: Acceptor. \<not> (is_safe A)
+                              \<and> FakeSend1b A st st2) \<or>
+                (\<exists>A :: Acceptor. \<not> (is_safe A)
+                              \<and> FakeSend2a A st st2)
+                "
+                using assms next_split by presburger
+    then show ?thesis
+    proof (elim disjE)
+      assume "ProposerSendAction st st2"
+      then show ?thesis
+        by (smt (verit) Msg_ref_Spec.elims(1) ProposerSendAction.elims(2) Send1a.elims(2) assms(1) assms(2) empty_iff next_msgs_preserved ref.simps(1) select_convs(1) set_ConsD subsetD subsetI surjective update_convs(1))
+    next
+      assume "\<exists>A. is_safe A \<and>
+                queued_msg st A = None \<and>
+                (\<exists>m\<in>set (msgs st).
+                    Process1a A m st st2)"
+      then show ?thesis
+      proof (clarify)
+        fix A m
+        assume "is_safe A"
+           and "queued_msg st A = None"
+           and "m \<in> set (msgs st)"
+           and "Process1a A m st st2"
+        define new1b where "new1b = M1b A (m # recent_msgs st A)"
+        show ?thesis
+        proof (cases "WellFormed st new1b")
+          case True
+          have "ref new1b \<subseteq> set (msgs st)"
+            by (metis KnownMsgs_accSpec.elims(2) RecentMsgsSpec.elims(2) \<open>is_safe A\<close> \<open>m \<in> set (msgs st)\<close> assms(3) assms(4) new1b_def ref.simps(2) set_ConsD subsetD subsetI)
+          have "msgs st2 = new1b # msgs st"
+            by (metis Process1a.elims(2) Send.elims(1) True \<open>Process1a A m st st2\<close> new1b_def)
+          then have "ref new1b \<subseteq> set (msgs st2)"
+            using \<open>ref new1b \<subseteq> set (msgs st)\<close> by auto
+          then show ?thesis
+            using \<open>msgs st2 = new1b # msgs st\<close> assms(2) by auto
+        next
+          case False
+          then show ?thesis
+            by (metis Msg_ref_Spec.elims(2) Msg_ref_Spec.elims(3) Process1a.elims(2) \<open>Process1a A m st st2\<close> assms(2) new1b_def)
+        qed
+      qed
+    next
+      assume "\<exists>A :: Acceptor. is_safe A
+                        \<and> queued_msg st A \<noteq> None 
+                        \<and> Process1b A (the (queued_msg st A)) st st2"
+      then show ?thesis
+        by (metis Msg_ref_Spec.elims(2) Msg_ref_Spec.elims(3) Process1b.elims(2) assms(2))
+
+    next
+      assume "\<exists>A :: Acceptor. is_safe A
+                  \<and> queued_msg st A = None 
+                  \<and> (\<exists>m \<in> set (msgs st). Process1b A m st st2)"
+      then show ?thesis
+        by (metis Msg_ref_Spec.simps Process1b.elims(2) assms(2))
+    next
+      assume "\<exists>A :: Acceptor. is_safe A
+                        \<and> two_a_lrn_loop st A 
+                        \<and> (\<exists>l :: Learner. Process1bLearnerLoopStep A l st st2)"
+      then show ?thesis
+      proof (clarify)
+        fix A l
+        assume "is_safe A"
+           and "two_a_lrn_loop st A"
+           and "Process1bLearnerLoopStep A l st st2"
+        define new2a where "new2a = M2a l A (recent_msgs st A)"
+        show ?thesis
+        proof (cases "WellFormed st new2a")
+          case True
+          then show ?thesis
+            by (smt (verit) KnownMsgs_accSpec.elims(2) Msg_ref_Spec.simps Process1bLearnerLoopStep.elims(2) RecentMsgsSpec.elims(2) Send.elims(2) \<open>Process1bLearnerLoopStep A l st st2\<close> \<open>is_safe A\<close> assms(2) assms(3) assms(4) in_mono list.set_intros(2) ref.simps(3) set_ConsD subsetI)
+        next
+          case False
+          then show ?thesis 
+            by (metis Msg_ref_Spec.simps Process1bLearnerLoopStep.elims(2) \<open>Process1bLearnerLoopStep A l st st2\<close> assms(2) new2a_def)
+        qed
+      qed
+    next
+      assume "\<exists>A. is_safe A \<and>
+        two_a_lrn_loop st A \<and>
+        Process1bLearnerLoopDone A st st2"
+      then show ?thesis
+        by (smt (verit) Msg_ref_Spec.simps Process1bLearnerLoopDone.elims(1) assms(2) ext_inject surjective update_convs(6))
+    next
+      assume "LearnerProcessAction st st2"
+      then show ?thesis
+        unfolding LearnerProcessAction.simps LearnerAction.simps
+      proof (clarify)
+        fix ln
+        assume "(\<exists>m\<in>set (msgs st). LearnerRecv ln m st st2) \<or>
+              (\<exists>blt val. LearnerDecide ln blt val st st2)"
+        then show ?thesis
+        proof (elim disjE; clarify)
+          fix m
+          assume "m \<in> set (msgs st)"
+             and "LearnerRecv ln m st st2"
+          then show ?thesis
+            unfolding LearnerRecv.simps
+          proof (cases "ln = l")
+            case True
+            have "known_msgs_lrn st2 l = m # known_msgs_lrn st l"
+              by (smt (verit, del_insts) LearnerRecv.elims(2) True \<open>LearnerRecv ln m st st2\<close> select_convs(3) surjective update_convs(3))
+            show ?thesis 
+              by (metis (no_types, lifting) LearnerRecv.elims(2) Msg_ref_Spec.simps \<open>LearnerRecv ln m st st2\<close> assms(2) select_convs(1) surjective update_convs(3))
+          next
+            case False
+            then show ?thesis
+              by (metis (no_types, lifting) LearnerRecv.elims(2) Msg_ref_Spec.simps \<open>LearnerRecv ln m st st2\<close> assms(2) select_convs(1) surjective update_convs(3))
+          qed
+          next
+            fix blt val
+            assume "LearnerDecide ln blt val st st2"
+            then show ?thesis
+              by (metis (no_types, lifting) LearnerDecide.elims(2) Msg_ref_Spec.simps assms(2) ext_inject surjective update_convs(8))
+        qed
+      qed
+    next
+      assume "\<exists>A. \<not> is_safe A \<and> FakeSend1b A st st2"
+      show ?thesis
+        by (smt (verit) FakeSend1b.elims(1) Msg_ref_Spec.simps \<open>\<exists>A. \<not> is_safe A \<and> FakeSend1b A st st2\<close> assms(2) hpaxos.acc.simps(2) list.set_intros(2) select_convs(1) set_ConsD subset_iff surjective update_convs(1))
+    next
+      assume "\<exists>A. \<not> is_safe A \<and> FakeSend2a A st st2"
+      then show ?thesis
+        unfolding FakeSend2a.simps Msg_ref_Spec.simps
+      proof (clarify)
+        fix m A fin ln x
+        assume "m \<in> set (msgs st2)"
+           and "\<not> is_safe A"
+           and "let new2a = M2a ln A fin
+               in WellFormed st new2a \<and>
+                  st2 = st\<lparr>msgs := new2a # msgs st\<rparr>"
+           and "is_safe (acc m)"
+           and "x \<in> ref m"
+        define new2a where "new2a = M2a ln A fin"
+        have "\<not> is_safe (acc new2a)"
+          by (simp add: \<open>\<not> is_safe A\<close> new2a_def)
+        have "\<forall>m \<in> set (msgs st2). is_safe (acc new2a) \<longrightarrow> m \<in> set (msgs st)"
+          using \<open>\<not> is_safe (acc new2a)\<close> by blast
+        have "m \<noteq> new2a"
+          using \<open>\<not> is_safe (acc new2a)\<close> \<open>is_safe (acc m)\<close> by blast
+        have "ref m \<subseteq> set (msgs st)"
+          by (metis Msg_ref_Spec.elims(2) \<open>is_safe (acc m)\<close> \<open>let new2a = M2a ln A fin in WellFormed st new2a \<and> st2 = st\<lparr>msgs := new2a # msgs st\<rparr>\<close> \<open>m \<in> set (msgs st2)\<close> \<open>m \<noteq> new2a\<close> assms(2) new2a_def select_convs(1) set_ConsD surjective update_convs(1))
+        then show "x \<in> set (msgs st2)"
+          using \<open>x \<in> ref m\<close> assms(1) next_msgs_preserved by blast
+      qed
+    qed
+qed
+
+lemma Msg_ref_Spec_Invariant:
+  assumes "Spec f"
+  shows "Msg_ref_Spec (f i)"
+proof (induction i)
+  case 0
+  then show ?case 
+    by (metis Init.elims Msg_ref_Spec.simps Spec.simps assms empty_iff empty_set select_convs(1))
+next
+  case (Suc i)
+  then show ?case
+    by (metis KnownMsgs_accSpecResult Msg_ref_Spec_Next RecentMsgsSpecResult Spec.elims(2) assms)
+qed
+
+
+fun WellFormed_Spec :: "State \<Rightarrow> bool" where
+  "WellFormed_Spec st = (
+    \<forall>m \<in> set (msgs st). is_safe (acc m) \<longrightarrow> WellFormed st m
+  )"
+
+lemma WellFormed_Spec_Next:
+  assumes "Next st st2"
+      and "WellFormed_Spec st"
+      and "KnownMsgs_accSpec st"
+    shows "WellFormed_Spec st2"
+proof -
+  have css: "ProposerSendAction st st2 \<or>
+                (\<exists>A :: Acceptor. is_safe A
+                            \<and> queued_msg st A = None 
+                            \<and> (\<exists>m \<in> set (msgs st). Process1a A m st st2)) \<or>
+                (\<exists>A :: Acceptor. is_safe A
+                              \<and> queued_msg st A \<noteq> None 
+                              \<and> Process1b A (the (queued_msg st A)) st st2) \<or>
+                (\<exists>A :: Acceptor. is_safe A
+                              \<and> queued_msg st A = None 
+                              \<and> (\<exists>m \<in> set (msgs st). Process1b A m st st2)) \<or>
+                (\<exists>A :: Acceptor. is_safe A
+                              \<and> two_a_lrn_loop st A 
+                              \<and> (\<exists>l :: Learner. Process1bLearnerLoopStep A l st st2)) \<or>
+                (\<exists>A :: Acceptor. is_safe A
+                              \<and> two_a_lrn_loop st A 
+                              \<and> Process1bLearnerLoopDone A st st2) \<or>
+                LearnerProcessAction st st2 \<or>
+                (\<exists>A :: Acceptor. \<not> (is_safe A)
+                              \<and> FakeSend1b A st st2) \<or>
+                (\<exists>A :: Acceptor. \<not> (is_safe A)
+                              \<and> FakeSend2a A st st2)
+                "
+                using assms next_split by presburger
+    then show ?thesis
+    proof (elim disjE)
+      assume "ProposerSendAction st st2"
+      then show ?thesis
+          by (smt (verit) MessageType.distinct(1) MessageType.distinct(3) ProposerSendAction.elims(2) Send1a.elims(2) WellFormed.elims(1) WellFormed_Spec.elims(1) Wellformed_Conservation_Next assms(1) assms(2) isValidMessage.simps(1) select_convs(1) set_ConsD surjective type.simps(1) update_convs(1))
+    next
+      assume "\<exists>A. is_safe A \<and>
+                queued_msg st A = None \<and>
+                (\<exists>m\<in>set (msgs st).
+                    Process1a A m st st2)"
+      then show ?thesis
+      proof (clarify)
+        fix A m
+        assume "is_safe A"
+           and "queued_msg st A = None"
+           and "m \<in> set (msgs st)"
+           and "Process1a A m st st2"
+        define new1b where "new1b = M1b A (m # recent_msgs st A)"
+        show ?thesis
+        proof (cases "WellFormed st new1b")
+          case True
+          then show ?thesis
+            by (smt (verit) Process1a.elims(2) Send.elims(2) WellFormed_Spec.elims(1) Wellformed_Conservation_Next \<open>Process1a A m st st2\<close> assms(1) assms(2) set_ConsD)
+        next
+          case False
+          then show ?thesis
+            by (metis Process1a.elims(2) WellFormed_Spec.elims(1) Wellformed_Conservation_Next \<open>Process1a A m st st2\<close> assms(1) assms(2) new1b_def)
+        qed
+      qed
+    next
+      assume "\<exists>A :: Acceptor. is_safe A
+                        \<and> queued_msg st A \<noteq> None 
+                        \<and> Process1b A (the (queued_msg st A)) st st2"
+      then show ?thesis
+        by (metis Process1b.elims(2) WellFormed_Spec.elims(2) WellFormed_Spec.elims(3) Wellformed_Conservation_Next assms(1) assms(2))
+    next
+      assume "\<exists>A :: Acceptor. is_safe A
+                  \<and> queued_msg st A = None 
+                  \<and> (\<exists>m \<in> set (msgs st). Process1b A m st st2)"
+      then show ?thesis
+      proof (clarify)
+        fix A m
+        assume "is_safe A"
+           and "queued_msg st A = None"
+           and "m \<in> set (msgs st)"
+        have "msgs st = msgs st2"
+          using \<open>\<exists>A. is_safe A \<and> queued_msg st A = None \<and> (\<exists>m\<in>set (msgs st). Process1b A m st st2)\<close> by fastforce
+        then show ?thesis
+          by (metis WellFormed_Spec.elims(1) Wellformed_Conservation_Next assms(1) assms(2))
+      qed
+    next
+      assume "\<exists>A :: Acceptor. is_safe A
+                        \<and> two_a_lrn_loop st A 
+                        \<and> (\<exists>l :: Learner. Process1bLearnerLoopStep A l st st2)"
+      then show ?thesis
+      proof (clarify)
+        fix A l
+        assume "is_safe A"
+           and "two_a_lrn_loop st A"
+           and "Process1bLearnerLoopStep A l st st2"
+        define new2a where "new2a = M2a l A (recent_msgs st A)"
+        show ?thesis
+        proof (cases "WellFormed st new2a")
+          case True
+          then show ?thesis
+            by (smt (verit) Process1bLearnerLoopStep.elims(2) Send.elims(2) WellFormed_Spec.elims(1) Wellformed_Conservation_Next \<open>Process1bLearnerLoopStep A l st st2\<close> assms(1) assms(2) set_ConsD)
+        next
+          case False
+          then show ?thesis 
+            by (metis Process1bLearnerLoopStep.elims(2) WellFormed_Spec.elims(1) Wellformed_Conservation_Next \<open>Process1bLearnerLoopStep A l st st2\<close> assms(1) assms(2) new2a_def)
+        qed
+      qed
+    next
+      assume "\<exists>A. is_safe A \<and>
+        two_a_lrn_loop st A \<and>
+        Process1bLearnerLoopDone A st st2"
+      then show ?thesis
+        by (metis (no_types, lifting) Process1bLearnerLoopDone.elims(1) WellFormed_Spec.elims(1) Wellformed_Conservation_Next assms(1) assms(2) select_convs(1) surjective update_convs(6))
+    next
+      assume "LearnerProcessAction st st2"
+      then show ?thesis
+        unfolding LearnerProcessAction.simps LearnerAction.simps
+      proof (clarify)
+        fix ln
+        assume "(\<exists>m\<in>set (msgs st). LearnerRecv ln m st st2) \<or>
+              (\<exists>blt val. LearnerDecide ln blt val st st2)"
+        then show ?thesis
+        proof (elim disjE; clarify)
+          fix m
+          assume "m \<in> set (msgs st)"
+             and "LearnerRecv ln m st st2"
+          then show ?thesis
+            by (metis (no_types, lifting) LearnerRecv.elims(2) WellFormed_Spec.elims(1) Wellformed_Conservation_Next assms(1) assms(2) select_convs(1) surjective update_convs(3))
+          next
+            fix blt val
+            assume "LearnerDecide ln blt val st st2"
+            then show ?thesis
+              by (metis (no_types, lifting) LearnerDecide.elims(2) WellFormed_Spec.elims(1) Wellformed_Conservation_Next assms(1) assms(2) select_convs(1) surjective update_convs(8))
+        qed
+      qed
+    next
+      assume "\<exists>A. \<not> is_safe A \<and> FakeSend1b A st st2"
+      show ?thesis
+        by (smt (z3) FakeSend1b.elims(1) WellFormed_Spec.elims(1) Wellformed_Conservation_Next \<open>\<exists>A. \<not> is_safe A \<and> FakeSend1b A st st2\<close> assms(1) assms(2) select_convs(1) set_ConsD surjective update_convs(1))
+    next
+      assume "\<exists>A. \<not> is_safe A \<and> FakeSend2a A st st2"
+      then show ?thesis
+        by (smt (z3) FakeSend2a.simps WellFormed_Spec.elims(1) Wellformed_Conservation_Next assms(1) assms(2) ext_inject set_ConsD surjective update_convs(1))
+    qed
+qed
+
+lemma WellFormed_Spec_Invariant:
+  assumes "Spec f"
+  shows "WellFormed_Spec (f i)"
+proof (induction i)
+  case 0
+  then show ?case 
+    by (metis Init.elims WellFormed_Spec.simps Spec.simps assms empty_iff empty_set select_convs(1))
+next
+  case (Suc i)
+  then show ?case
+    by (metis KnownMsgs_accSpecResult WellFormed_Spec_Next Spec.elims(2) assms)
+qed
+
+
+fun Enabled :: "(State \<Rightarrow> State \<Rightarrow> bool) \<Rightarrow> State \<Rightarrow> bool" where
+  "Enabled r st = (\<exists>st2. r st st2)"
+
+lemma Exists_Enabled_Swap:
+  shows "Enabled (\<lambda>st st2. \<exists>v. R v st st2) s = (\<exists>v. Enabled (R v) s)"  
+  by auto
+
+(* Send1a is always enabled.*)
+lemma Send1a_Enabled:
+  shows "Enabled (Send1a b) st = True"
+  by fastforce
+
+lemma Process1aAlt1:
+  assumes "WellFormed st (M1b a (m # recent_msgs st a))"
+      and "type m = T1a"
+      and "Recv_acc st a m"
+    shows "Process1a a m st (st\<lparr>msgs := M1b a (m # recent_msgs st a) # msgs st, 
+                                recent_msgs := (
+                                  \<lambda>a2. if a2 = a then [] 
+                                                 else recent_msgs st a2),
+                                queued_msg := (
+                                  \<lambda>a2. if a2 = a then Some (M1b a (m # recent_msgs st a)) 
+                                                 else queued_msg st a2),
+                                known_msgs_acc := (
+                                  \<lambda>x. if a = x 
+                                      then m # known_msgs_acc st x
+                                      else known_msgs_acc st x) \<rparr>)"
+proof -
+  define st2 where "st2 = (st\<lparr>msgs := M1b a (m # recent_msgs st a) # msgs st, 
+                              recent_msgs := (
+                                \<lambda>a2. if a2 = a then [] 
+                                               else recent_msgs st a2),
+                              queued_msg := (
+                                \<lambda>a2. if a2 = a then Some (M1b a (m # recent_msgs st a)) 
+                                               else queued_msg st a2),
+                              known_msgs_acc := (
+                                \<lambda>x. if a = x 
+                                    then m # known_msgs_acc st x
+                                    else known_msgs_acc st x) \<rparr>)"
+  
+  have "Store_acc a m st st2" 
+    by (simp add: st2_def)
+  have "Send (M1b a (m # recent_msgs st a)) st st2
+          \<and> (recent_msgs st2 = (
+              \<lambda>a2. if a2 = a then [] 
+                             else recent_msgs st a2))
+          \<and> (queued_msg st2 = (
+              \<lambda>a2. if a2 = a then Some (M1b a (m # recent_msgs st a)) 
+                             else queued_msg st a2))"
+    by (simp add: st2_def)
+  show ?thesis
+    unfolding Process1a.simps
+    by (smt (verit, ccfv_SIG) \<open>Send (M1b a (m # recent_msgs st a)) st st2 \<and> recent_msgs st2 = (\<lambda>a2. if a2 = a then [] else recent_msgs st a2) \<and> queued_msg st2 = (\<lambda>a2. if a2 = a then Some (M1b a (m # recent_msgs st a)) else queued_msg st a2)\<close> \<open>Store_acc a m st st2\<close> assms(1) assms(2) assms(3) ext_inject st2_def surjective update_convs(1) update_convs(2) update_convs(4) update_convs(5))
+qed
+
+lemma Process1aAlt2:
+  assumes "\<not> WellFormed st (M1b a (m # recent_msgs st a))"
+      and "type m = T1a"
+      and "Recv_acc st a m"
+    shows "Process1a a m st (st\<lparr>recent_msgs := (
+                              \<lambda>a2. if a2 = a then m # recent_msgs st a2 
+                                             else recent_msgs st a2),
+                            known_msgs_acc := (
+                                \<lambda>x. if a = x 
+                                    then m # known_msgs_acc st x
+                                    else known_msgs_acc st x)\<rparr>)"
+proof -
+  define st2 where "st2 = (st\<lparr>recent_msgs := (
+                              \<lambda>a2. if a2 = a then m # recent_msgs st a2 
+                                             else recent_msgs st a2),
+                            known_msgs_acc := (
+                                \<lambda>x. if a = x 
+                                    then m # known_msgs_acc st x
+                                    else known_msgs_acc st x)\<rparr>)"
+  
+  have "Store_acc a m st st2" 
+    by (simp add: st2_def)
+  have "(recent_msgs st2 = (
+              \<lambda>a2. if a2 = a then m # recent_msgs st a2 
+                             else recent_msgs st a2))
+          \<and> (msgs st = msgs st2)
+          \<and> (queued_msg st = queued_msg st2)"
+    by (simp add: st2_def)
+  show ?thesis
+    unfolding Process1a.simps
+    using assms(1) assms(2) assms(3) by auto
+qed
+
+lemma Process1a_Enabled:
+  shows "Enabled (Process1a a m) st = (type m = T1a \<and> Recv_acc st a m)"
+  by (metis (no_types, lifting) Enabled.simps Process1a.simps Process1aAlt1 Process1aAlt2)
+
+lemma Process1a_Trans:
+  assumes "m \<notin> set (known_msgs_acc st a2)"
+      and "Enabled (Process1a a1 m) st"
+    shows "Enabled (Process1a a2 m) st"
+  by (metis MessageType.distinct(1) MessageType.distinct(3) Process1a_Enabled Proper_acc.elims(1) Recv_acc.elims(2) Recv_acc.elims(3) assms(1) assms(2) empty_iff ref.simps(1) type.elims)
+
+lemma Process1bAlt1:
+  assumes "\<forall> mb b :: Ballot. MaxBal st a b \<and> B m b \<longrightarrow> mb \<le> b"
+      and "type m = T1b"
+      and "Recv_acc st a m"
+    shows "Process1b a m st (st\<lparr>recent_msgs := (
+                                      \<lambda>x. if x = a 
+                                          then m # recent_msgs st x
+                                          else recent_msgs st x ),
+                                known_msgs_acc := (
+                                  \<lambda>x. if a = x 
+                                      then m # known_msgs_acc st x
+                                      else known_msgs_acc st x),
+                                two_a_lrn_loop := (\<lambda>x.
+                                    if x = a
+                                    then True
+                                    else two_a_lrn_loop st x),
+                                 processed_lrns := (\<lambda>x.
+                                      if x = a
+                                      then {}
+                                      else processed_lrns st x),
+                                queued_msg := (\<lambda>x.
+                                      if x = a
+                                      then None
+                                      else queued_msg st x) \<rparr>)"
+proof -
+  define st2 where "st2 = st\<lparr>recent_msgs := (
+                                      \<lambda>x. if x = a 
+                                          then m # recent_msgs st x
+                                          else recent_msgs st x ),
+                            known_msgs_acc := (
+                              \<lambda>x. if a = x 
+                                  then m # known_msgs_acc st x
+                                  else known_msgs_acc st x),
+                            two_a_lrn_loop := (\<lambda>x.
+                                if x = a
+                                then True
+                                else two_a_lrn_loop st x),
+                             processed_lrns := (\<lambda>x.
+                                  if x = a
+                                  then {}
+                                  else processed_lrns st x),
+                            queued_msg := (\<lambda>x.
+                                  if x = a
+                                  then None
+                                  else queued_msg st x) \<rparr>"
+  have "recent_msgs st2 = (
+        \<lambda>x. if x = a 
+            then m # recent_msgs st x
+            else recent_msgs st x )" by (simp add: st2_def)
+  have "queued_msg st2 = (\<lambda>x.
+          if x = a
+          then None
+          else queued_msg st x)" by (simp add: st2_def)
+  have "Store_acc a m st st2" by (simp add: st2_def)
+  have "two_a_lrn_loop st2 = (\<lambda>x.
+          if x = a
+          then True
+          else two_a_lrn_loop st x)
+        \<and> processed_lrns st2 = (\<lambda>x.
+          if x = a
+          then {}
+          else processed_lrns st x)" by (simp add: st2_def)
+  have "(msgs st2 = msgs st)
+    \<and> (decision st2 = decision st)
+    \<and> (BVal st2 = BVal st)" by (simp add: st2_def)
+  show ?thesis
+    unfolding Process1b.simps
+    using \<open>Store_acc a m st st2\<close> \<open>msgs st2 = msgs st \<and> decision st2 = decision st \<and> BVal st2 = BVal st\<close> \<open>queued_msg st2 = (\<lambda>x. if x = a then None else queued_msg st x)\<close> \<open>recent_msgs st2 = (\<lambda>x. if x = a then m # recent_msgs st x else recent_msgs st x)\<close> \<open>two_a_lrn_loop st2 = (\<lambda>x. if x = a then True else two_a_lrn_loop st x) \<and> processed_lrns st2 = (\<lambda>x. if x = a then {} else processed_lrns st x)\<close> assms(1) assms(2) assms(3) st2_def by fastforce
+qed
+
+lemma Process1bAlt2:
+  assumes "\<not> (\<forall> mb b :: Ballot. MaxBal st a b \<and> B m b \<longrightarrow> mb \<le> b)"
+      and "type m = T1b"
+      and "Recv_acc st a m"
+    shows "Process1b a m st (st\<lparr>recent_msgs := (
+                                      \<lambda>x. if x = a 
+                                          then m # recent_msgs st x
+                                          else recent_msgs st x ),
+                                known_msgs_acc := (
+                                  \<lambda>x. if a = x 
+                                      then m # known_msgs_acc st x
+                                      else known_msgs_acc st x),
+                                queued_msg := (\<lambda>x.
+                                      if x = a
+                                      then None
+                                      else queued_msg st x) \<rparr>)"
+proof -
+  define st2 where "st2 = st\<lparr>recent_msgs := (
+                                      \<lambda>x. if x = a 
+                                          then m # recent_msgs st x
+                                          else recent_msgs st x ),
+                            known_msgs_acc := (
+                              \<lambda>x. if a = x 
+                                  then m # known_msgs_acc st x
+                                  else known_msgs_acc st x),
+                            queued_msg := (\<lambda>x.
+                                  if x = a
+                                  then None
+                                  else queued_msg st x) \<rparr>"
+  have "recent_msgs st2 = (
+        \<lambda>x. if x = a 
+            then m # recent_msgs st x
+            else recent_msgs st x )" by (simp add: st2_def)
+  have "queued_msg st2 = (\<lambda>x.
+          if x = a
+          then None
+          else queued_msg st x)" by (simp add: st2_def)
+  have "Store_acc a m st st2" by (simp add: st2_def)
+  have "two_a_lrn_loop st2 = two_a_lrn_loop st
+        \<and> processed_lrns st2 = processed_lrns st" by (simp add: st2_def)
+  have "(msgs st2 = msgs st)
+    \<and> (decision st2 = decision st)
+    \<and> (BVal st2 = BVal st)" by (simp add: st2_def)
+  show ?thesis
+    unfolding Process1b.simps
+    using \<open>Store_acc a m st st2\<close> \<open>msgs st2 = msgs st \<and> decision st2 = decision st \<and> BVal st2 = BVal st\<close> \<open>queued_msg st2 = (\<lambda>x. if x = a then None else queued_msg st x)\<close> \<open>recent_msgs st2 = (\<lambda>x. if x = a then m # recent_msgs st x else recent_msgs st x)\<close> \<open>two_a_lrn_loop st2 = two_a_lrn_loop st \<and> processed_lrns st2 = processed_lrns st\<close> assms(1) assms(2) assms(3) st2_def by blast
+qed
+
+lemma Process1b_Enabled:
+  shows "Enabled (Process1b a m) st = (type m = T1b \<and> Recv_acc st a m)"
+  by (smt (verit, best) Enabled.simps Process1b.simps Process1bAlt1 Process1bAlt2)
+
+lemma Process2aAlt:
+  assumes "type m = T2a"
+      and "Recv_acc st a m"
+    shows "Process2a a m st (st\<lparr>recent_msgs := (
+                                  \<lambda>x. if x = a 
+                                      then m # recent_msgs st x
+                                      else recent_msgs st x ),
+                                known_msgs_acc := (
+                                      \<lambda>x. if a = x 
+                                          then m # known_msgs_acc st x
+                                          else known_msgs_acc st x
+                                  )\<rparr>)"
+proof -
+  define st2 where "st2 = st\<lparr>recent_msgs := (
+                                  \<lambda>x. if x = a 
+                                      then m # recent_msgs st x
+                                      else recent_msgs st x ),
+                              known_msgs_acc := (
+                                    \<lambda>x. if a = x 
+                                        then m # known_msgs_acc st x
+                                        else known_msgs_acc st x
+                                )\<rparr>"
+  have "Store_acc a m st st2
+    \<and> recent_msgs st2 = (
+        \<lambda>x. if x = a 
+            then m # recent_msgs st x
+            else recent_msgs st x )
+    \<and> (msgs st2 = msgs st)
+    \<and> (queued_msg st2 = queued_msg st)
+    \<and> (two_a_lrn_loop st2 = two_a_lrn_loop st)
+    \<and> (processed_lrns st2 = processed_lrns st)
+    \<and> (decision st2 = decision st)
+    \<and> (BVal st2 = BVal st)" by (simp add: st2_def)
+  show ?thesis
+    unfolding Process2a.simps
+    using \<open>Store_acc a m st st2 \<and> recent_msgs st2 = (\<lambda>x. if x = a then m # recent_msgs st x else recent_msgs st x) \<and> msgs st2 = msgs st \<and> queued_msg st2 = queued_msg st \<and> two_a_lrn_loop st2 = two_a_lrn_loop st \<and> processed_lrns st2 = processed_lrns st \<and> decision st2 = decision st \<and> BVal st2 = BVal st\<close> assms(1) assms(2) st2_def by fastforce
+qed
+
+lemma Process2a_Enabled:
+  shows "Enabled (Process2a a m) st = (type m = T2a \<and> Recv_acc st a m)"
+  by (metis (no_types, lifting) Enabled.simps Process2a.simps Process2aAlt)
+
+lemma Process1bLearnerLoopStepAlt1:
+  assumes "WellFormed st (M2a ln a (recent_msgs st a))"
+  shows "Process1bLearnerLoopStep a ln st (
+                              st\<lparr>processed_lrns := (
+                                    \<lambda>x . if x = a
+                                         then {ln} \<union> processed_lrns st x
+                                         else processed_lrns st x),
+                                msgs := M2a ln a (recent_msgs st a) # msgs st, 
+                                known_msgs_acc := (
+                                    \<lambda>x. if a = x 
+                                        then M2a ln a (recent_msgs st a) # known_msgs_acc st x
+                                        else known_msgs_acc st x),
+                                recent_msgs := (
+                                    \<lambda>x . if x = a
+                                       then [M2a ln a (recent_msgs st a)]
+                                       else recent_msgs st x) \<rparr>)"
+proof -
+  define new2a where "new2a = M2a ln a (recent_msgs st a)"
+  define st2 where "st2 = (st\<lparr>processed_lrns := (
+                                    \<lambda>x . if x = a
+                                         then {ln} \<union> processed_lrns st x
+                                         else processed_lrns st x),
+                                msgs := new2a # msgs st, 
+                                known_msgs_acc := (
+                                    \<lambda>x. if a = x 
+                                        then new2a # known_msgs_acc st x
+                                        else known_msgs_acc st x),
+                                recent_msgs := (
+                                    \<lambda>x . if x = a
+                                       then [new2a]
+                                       else recent_msgs st x) \<rparr>)"
+  have "Send new2a st st2
+          \<and> Store_acc a new2a st st2
+          \<and> (recent_msgs st2 = (
+              \<lambda>x . if x = a
+                 then [new2a]
+                 else recent_msgs st x))" 
+    by (simp add: st2_def)
+  have "processed_lrns st2 = (
+          \<lambda>x . if x = a
+               then {ln} \<union> processed_lrns st x
+               else processed_lrns st x)" 
+    by (simp add: st2_def)
+  have "(queued_msg st2 = queued_msg st)
+          \<and> (two_a_lrn_loop st2 = two_a_lrn_loop st)
+          \<and> (decision st2 = decision st)
+          \<and> (BVal st2 = BVal st)" 
+    by (simp add: st2_def)
+  show ?thesis
+    unfolding Process1bLearnerLoopStep.simps simps
+    using assms by force
+qed
+
+lemma Process1bLearnerLoopStepAlt2:
+  assumes "\<not> WellFormed st (M2a ln a (recent_msgs st a))"
+  shows "Process1bLearnerLoopStep a ln st (
+                        st\<lparr>processed_lrns := (
+                                    \<lambda>x . if x = a
+                                         then {ln} \<union> processed_lrns st x
+                                         else processed_lrns st x)\<rparr>)"
+proof -
+  define st2 where "st2 = st\<lparr>processed_lrns := (
+                                    \<lambda>x . if x = a
+                                         then {ln} \<union> processed_lrns st x
+                                         else processed_lrns st x)\<rparr>"
+  have "processed_lrns st2 = (
+          \<lambda>x . if x = a
+               then {ln} \<union> processed_lrns st x
+               else processed_lrns st x)" 
+    by (simp add: st2_def)
+  have "(msgs st2 = msgs st)
+          \<and> (known_msgs_acc st2 = known_msgs_acc st)
+          \<and> (known_msgs_lrn st2 = known_msgs_lrn st)
+          \<and> (recent_msgs st2 = recent_msgs st)" 
+    by (simp add: st2_def)
+  have "(queued_msg st2 = queued_msg st)
+          \<and> (two_a_lrn_loop st2 = two_a_lrn_loop st)
+          \<and> (decision st2 = decision st)
+          \<and> (BVal st2 = BVal st)" 
+    by (simp add: st2_def)
+  show ?thesis
+    unfolding Process1bLearnerLoopStep.simps
+    using assms by force
+qed
+
+lemma Process1bLearnerLoopStep_Enabled:
+  "Enabled (Process1bLearnerLoopStep a l) st = True"
+  by (meson Enabled.elims(3) Process1bLearnerLoopStepAlt1 Process1bLearnerLoopStepAlt2)
+
+lemma Process1bLearnerLoopDone_Enabled:
+  "Enabled (Process1bLearnerLoopDone a) st = (\<forall>ln :: Learner. ln \<in> processed_lrns st a)"
+  by auto
+
+(* Process1bLearnerLoop is always enabled.*)
+lemma Process1bLearnerLoop_Enabled:
+  "Enabled (Process1bLearnerLoop a) st = True"
+  by (metis Enabled.elims(1) Process1bLearnerLoop.elims(3) Process1bLearnerLoopDone_Enabled Process1bLearnerLoopStep_Enabled)
+
+lemma AcceptorAction_Enabled:
+  shows "Enabled (AcceptorAction a) st = (
+    is_safe a \<and> (
+      (\<not> two_a_lrn_loop st a \<and>
+       ((queued_msg st a \<noteq> None \<and> 
+         type (the (queued_msg st a)) = T1b \<and> 
+         Recv_acc st a (the (queued_msg st a))) \<or> 
+        (queued_msg st a = None \<and> (
+          \<exists>m \<in> set (msgs st). Recv_acc st a m \<and> (type m = T1a \<or> type m = T1b)
+        ))))
+      \<or> two_a_lrn_loop st a)
+  )"
+  by (metis AcceptorAction.simps Enabled.elims(1) Process1a_Enabled Process1bLearnerLoop_Enabled Process1b_Enabled)
+
+lemma AcceptorAction_NotEnabled:
+  assumes "is_safe a"
+  shows "\<not> Enabled (AcceptorAction a) st = (
+     (queued_msg st a = None \<or> 
+        type (the (queued_msg st a)) \<noteq> T1b \<or> 
+        \<not> Recv_acc st a (the (queued_msg st a))) \<and> 
+     (queued_msg st a \<noteq> None \<or> (
+         \<forall>m \<in> set (msgs st). \<not> Recv_acc st a m \<or> (type m \<noteq> T1a \<and> type m \<noteq> T1b)
+     ))
+     \<and> \<not> two_a_lrn_loop st a
+  )"
+  by (metis AcceptorAction_Enabled assms)
+
+
+lemma AcceptorAction_NotEnabled_Spec:
+  assumes "Spec f"
+      and "is_safe a"
+  shows "\<not> Enabled (AcceptorAction a) (f i) = (
+     (queued_msg (f i) a = None)
+     \<and> \<not> (\<exists>m \<in> set (msgs (f i)). Recv_acc (f i) a m \<and> (type m = T1a \<or> type m = T1b))
+     \<and> \<not> two_a_lrn_loop (f i) a
+  )"
+  by (metis AcceptorAction_NotEnabled QueuedMsgResult QueuedMsgSpec1.elims(2) QueuedMsgSpec2.elims(2) QueuedMsgSpec2_Conserved assms(1) assms(2))
+
+lemma LearnerRecv_Enabled:
+  shows "Enabled (LearnerRecv l m) st = Recv_lrn st l m"
+  using Enabled.simps LearnerRecv.simps by presburger
+
+lemma LearnerDecide_Enabled:
+  shows "Enabled (LearnerDecide l b v) st = ChosenIn st l b v"
+  using Enabled.simps LearnerDecide.simps by presburger
+
+lemma LearnerAction_Enabled:
+  shows "Enabled (LearnerAction l) st = (
+      (\<exists>m\<in>set (msgs st). Recv_lrn st l m) \<or> 
+      (\<exists>b v. ChosenIn st l b v))"
+  by (metis Enabled.simps LearnerAction.elims(2) LearnerAction.elims(3) LearnerDecide_Enabled LearnerRecv_Enabled)
+
+
+
+(*Weak fairness*)
+fun WF :: "(State \<Rightarrow> State \<Rightarrow> bool) \<Rightarrow> (nat \<Rightarrow> State) \<Rightarrow> bool" where
+  "WF p f = (
+    \<forall>i. (\<forall>j \<ge> i. Enabled p (f j)) \<longrightarrow> (\<exists>j \<ge> i. p (f j) (f (1 + j)))
+  )"
+
+
+
+lemma Learner_Eventually_Gets_All_Safe_Messages:
+  assumes "Spec f"
+      and "\<forall>m\<in>set (msgs (f i)). \<not> Enabled (LearnerRecv L m) (f i)"
+    shows "m\<in>set (msgs (f i)) \<and> is_safe (acc m) \<longrightarrow> m \<in> set (known_msgs_lrn (f i) L)"
+proof (induction m; clarify)
+  case (M1a x)
+  assume "M1a x \<in> set (msgs (f i))"
+  have "\<not> Enabled (LearnerRecv L (M1a x)) (f i)"
+    using \<open>M1a x \<in> set (msgs (f i))\<close> assms(2) by blast
+  then show "M1a x \<in> set (known_msgs_lrn (f i) L)" 
+    by (metis LearnerRecv_Enabled M1a_Good MessageType.distinct(1) MessageType.distinct(3) Recv_lrn.elims(1) WellFormed.elims(1) \<open>M1a x \<in> set (msgs (f i))\<close> isValidMessage.simps(1) type.simps(1))
+next
+  case (M1b x1a x2)
+  assume "(\<And>x2a. x2a \<in> set x2 \<Longrightarrow>
+               x2a \<in> set (msgs (f i)) \<and>
+               is_safe (acc x2a) \<longrightarrow>
+               x2a \<in> set (known_msgs_lrn (f i) L))"
+      and "M1b x1a x2 \<in> set (msgs (f i))"
+      and "is_safe (acc (M1b x1a x2))"
+  have "WellFormed (f i) (M1b x1a x2)"
+    using WellFormed_Spec.simps WellFormed_Spec_Invariant \<open>M1b x1a x2 \<in> set (msgs (f i))\<close> \<open>is_safe (acc (M1b x1a x2))\<close> assms(1) by blast
+  then have "\<forall>y\<in>Tran (M1b x1a x2). M1b x1a x2 \<noteq> y \<and> SameBallot (M1b x1a x2) y \<longrightarrow> type y = T1a"
+    by (meson WellFormed.elims(2) type.simps(2))
+  have "\<not> Enabled (LearnerRecv L (M1b x1a x2)) (f i)"
+    using \<open>M1b x1a x2 \<in> set (msgs (f i))\<close> assms(2) by blast
+  then have "\<not> Recv_lrn (f i) L (M1b x1a x2)"    
+    using LearnerRecv_Enabled by blast
+  have "\<forall>r\<in>set x2. is_safe (acc r)"
+    sorry
+  then have "Proper_lrn (f i) L (M1b x1a x2)"
+    unfolding Proper_lrn.simps ref.simps
+    sorry
+
+  then show "M1b x1a x2 \<in> set (known_msgs_lrn (f i) L)" sorry
+next
+  case (M2a x1a x2 x3)
+  assume "(\<And>x3a. x3a \<in> set x3 \<Longrightarrow>
+               x3a \<in> set (msgs (f i)) \<and>
+               is_safe (acc x3a) \<longrightarrow>
+               x3a \<in> set (known_msgs_lrn (f i) L))"
+      and "M2a x1a x2 x3 \<in> set (msgs (f i))"
+      and "is_safe (acc (M2a x1a x2 x3))"
+  then show "M2a x1a x2 x3 \<in> set (known_msgs_lrn (f i) L)" sorry
+qed
+
+
+
+
+
+
+end
